more reorganization

theories/aneris_lang/lib/list.v
@@ -3,151 +3,145 @@ From aneris.aneris_lang Require Import lang proofmode notation.
 Set Default Proof Using "Type".
 
 Import Network.
-Import String.
-Import uPred.
 
-Module List.
+Definition list_nil : base_lang.expr := NONE.
 
-  Definition nil : base_lang.expr := NONE.
+Definition list_cons : base_lang.val :=
+  λ: "elem" "list", SOME (Pair "elem" "list").
 
-  Definition cons : base_lang.val :=
-    λ: "elem" "list", SOME (Pair "elem" "list").
+Definition list_head : base_lang.val :=
+  λ: "l", match: "l" with
+            SOME "a" => SOME (Fst "a")
+          | NONE => NONE
+          end.
 
-  Definition head : base_lang.val :=
-    λ: "l", match: "l" with
-              SOME "a" => SOME (Fst "a")
-            | NONE => NONE
-            end.
+Definition list_tail : base_lang.val :=
+  λ: "l", match: "l" with
+            SOME "a" => (Snd "a")
+          | NONE => NONE
+          end.
 
-  Definition tail : base_lang.val :=
-    λ: "l", match: "l" with
-              SOME "a" => (Snd "a")
-            | NONE => NONE
-            end.
+Definition list_fold : base_lang.val :=
+  rec: "fold" "handler" "acc" "l" :=
+    match: "l" with
+      SOME "a" => let: "fst" := Fst "a" in
+                  let: "snd" := Snd "a" in
+                  let: "acc'" := ("handler" "acc" "fst") in
+                  "fold" "handler" "acc'" "snd"
+    | NONE => "acc"
+    end.
 
-  Definition fold : base_lang.val :=
-    rec: "fold" "handler" "acc" "l" :=
+Definition list_iter : base_lang.val :=
+  rec: "iter" "handler" "l" :=
+    match: "l" with
+      SOME "a" =>
+      let: "tail" := Snd "a" in
+      "handler" (Fst "a");;
+      "iter" "handler" "tail"
+    | NONE => #()
+    end.
+
+Definition list_length : base_lang.val :=
+  rec: "length" "l" :=
+    match: "l" with
+      SOME "a" => #1 + "length" (Snd "a")
+    | NONE => #0
+    end.
+
+Definition list_nth : base_lang.val :=
+  (rec: "nth" "l" "i" :=
+     match: "l" with
+       SOME "a" =>
+       if: "i" = #0 then SOME (Fst "a")
+       else "nth" (Snd "a") ("i" - #1)
+     | NONE => NONE
+     end)%V.
+
+Definition list_find_remove : base_lang.val :=
+  (rec: "find" "f" "l" :=
+     match: "l" with
+       SOME "a" =>
+       let: "head" := Fst "a" in
+       let: "tail" := Snd "a" in
+       if: "f" "head" then SOME ("head", "tail")
+       else
+         let: "r" := "find" "f" "tail" in
+         match: "r" with
+           SOME "b" =>
+           let: "head'" := Fst "b" in
+           let: "tail'" := Snd "b" in
+           SOME ("head'", list_cons "head" "tail'")
+         | NONE => NONE
+         end
+     | NONE => NONE
+     end).
+
+Definition list_sub : base_lang.val :=
+  rec: "sub" "i" "l" :=
+    if: "i" = #0 then NONEV
+    else
       match: "l" with
-        SOME "a" => let: "fst" := Fst "a" in
-                   let: "snd" := Snd "a" in
-                   let: "acc'" := ("handler" "acc" "fst") in
-                   "fold" "handler" "acc'" "snd"
-      | NONE => "acc"
+        SOME "a" => list_cons (Fst "a") ("sub" ("i" - #1) (Snd "a"))
+      | NONE => NONEV
       end.
 
-  Definition iter : base_lang.val :=
-    rec: "iter" "handler" "l" :=
-      match: "l" with
-        SOME "a" =>
-        let: "tail" := Snd "a" in
-        "handler" (Fst "a");;
-                  "iter" "handler" "tail"
-      | NONE => #()
-      end.
-
-  Definition length : base_lang.val :=
-    rec: "length" "l" :=
-      match: "l" with
-        SOME "a" => #1 + "length" (Snd "a")
-      | NONE => #0
-      end.
-
-  Definition nth : base_lang.val :=
-    (rec: "nth" "l" "i" :=
-      match: "l" with
-        SOME "a" =>
-        if: "i" = #0 then SOME (Fst "a")
-        else "nth" (Snd "a") ("i" - #1)
-      | NONE => NONE
-      end)%V.
-
-  Definition find_remove : base_lang.val :=
-    (rec: "find" "f" "l" :=
-       match: "l" with
-         SOME "a" =>
-           let: "head" := Fst "a" in
-           let: "tail" := Snd "a" in
-           if: "f" "head" then SOME ("head", "tail")
-           else
-             let: "r" := "find" "f" "tail" in
-             match: "r" with
-               SOME "b" =>
-                 let: "head'" := Fst "b" in
-                 let: "tail'" := Snd "b" in
-                 SOME ("head'", cons "head" "tail'")
-             | NONE => NONE
-             end
-       | NONE => NONE
-       end).
-
-  Definition sub : base_lang.val :=
-    rec: "sub" "i" "l" :=
-      if: "i" = #0 then NONEV
-      else
-        match: "l" with
-          SOME "a" => cons (Fst "a") ("sub" ("i" - #1) (Snd "a"))
-        | NONE => NONEV
-        end.
-
-  Definition rev_aux : base_lang.val :=
+Definition list_rev_aux : base_lang.val :=
   rec: "rev_aux" "l" "acc" :=
     match: "l" with
       NONE => "acc"
     | SOME "p" =>
-       let: "h" := Fst "p" in
-       let: "t" := Snd "p" in
-       let: "acc'" := cons "h" "acc" in
-       "rev_aux" "t" "acc'"
+      let: "h" := Fst "p" in
+      let: "t" := Snd "p" in
+      let: "acc'" := list_cons "h" "acc" in
+      "rev_aux" "t" "acc'"
     end.
 
-  Definition rev : base_lang.val :=
-    λ: "l", rev_aux "l" NONE.
+Definition list_rev : base_lang.val :=
+  λ: "l", list_rev_aux "l" NONE.
 
-  Definition append : base_lang.val :=
-    (rec: "append" "l" "r" :=
-      match: "l" with
-      NONE => "r"
-    | SOME "p" =>
+Definition list_append : base_lang.val :=
+  (rec: "append" "l" "r" :=
+     match: "l" with
+       NONE => "r"
+     | SOME "p" =>
        let: "h" := Fst "p" in
        let: "t" := Snd "p" in
-       cons "h" ("append" "t" "r")
-    end)%V.
+       list_cons "h" ("append" "t" "r")
+     end)%V.
 
-  Definition is_empty : base_lang.val :=
-    λ: "l", match: "l" with
-              NONE => #true
-            | SOME "x" => #false
-            end.
-End List.
+Definition list_is_empty : base_lang.val :=
+  λ: "l", match: "l" with
+            NONE => #true
+          | SOME "x" => #false
+          end.
 
-Section List_specs.
+Section list_specs.
   Context `{dG : anerisG Mdl Σ}.
-  Import List.
 
-  Fixpoint is_List l v :=
+  Fixpoint is_list l v :=
     match l with
     | [] => v = NONEV
-    | a::l' => ∃ lv : base_lang.val, v = SOMEV (a,lv) ∧ is_List l' lv
+    | a::l' => ∃ lv : base_lang.val, v = SOMEV (a,lv) ∧ is_list l' lv
   end.
 
-  Lemma list_nil_spec ip :
+  Lemma wp_list_nil ip :
     {{{ True }}}
-      nil @[ip]
-    {{{ v, RET v; ⌜is_List [] v⌝}}}.
+      list_nil @[ip]
+    {{{ v, RET v; ⌜is_list [] v⌝}}}.
   Proof. iIntros (Φ) "_ HΦ". wp_pures. by iApply "HΦ". Qed.
 
-  Lemma list_cons_spec ip a lv l :
-    {{{ ⌜is_List l lv⌝ }}}
-      cons (Val a) (Val lv) @[ip]
-    {{{ v, RET v; ⌜is_List (a::l) v⌝}}}.
+  Lemma wp_list_cons l lv ip a :
+    {{{ ⌜is_list l lv⌝ }}}
+      list_cons (Val a) (Val lv) @[ip]
+    {{{ v, RET v; ⌜is_list (a::l) v⌝}}}.
   Proof.
     iIntros (Φ) "% HΦ". wp_lam. wp_pures.
     iApply "HΦ". iPureIntro; by eexists.
   Qed.
 
-  Lemma list_head_spec ip lv l :
-    {{{ ⌜is_List l lv⌝ }}}
-      head (Val lv) @[ip]
+  Lemma wp_list_head ip lv l :
+    {{{ ⌜is_list l lv⌝ }}}
+      list_head (Val lv) @[ip]
     {{{ v, RET v;
         ⌜(l = [] ∧ v = NONEV) ∨ (∃ v' l', l = v' :: l' ∧ v = SOMEV v')⌝ }}}.
   Proof.
@@ -158,10 +152,10 @@ Section List_specs.
       wp_pures. iApply "HΦ". iPureIntro. right. by exists v,l.
   Qed.
 
-  Lemma list_tail_spec ip lv l :
-    {{{ ⌜is_List l lv⌝ }}}
-      tail (Val lv) @[ip]
-    {{{ v, RET v; ⌜is_List (list.tail l) v⌝}}}.
+  Lemma wp_list_tail ip lv l :
+    {{{ ⌜is_list l lv⌝ }}}
+      list_tail (Val lv) @[ip]
+    {{{ v, RET v; ⌜is_list (tail l) v⌝}}}.
   Proof.
     iIntros (Φ a) "HΦ".
     wp_lam. destruct l; simpl in *; subst.
@@ -170,33 +164,33 @@ Section List_specs.
       wp_match. wp_proj. by iApply "HΦ".
   Qed.
 
-  Lemma list_length_spec ip l lv :
-    {{{ ⌜is_List l lv⌝ }}}
-      length (Val lv) @[ip]
-    {{{ v, RET #v; ⌜v = Datatypes.length l⌝ }}}.
+  Lemma wp_list_length ip l lv :
+    {{{ ⌜is_list l lv⌝ }}}
+      list_length (Val lv) @[ip]
+    {{{ v, RET #v; ⌜v = length l⌝ }}}.
   Proof.
     iIntros (Φ) "Ha HΦ".
     iInduction l as [|a l'] "IH" forall (lv Φ);
     iDestruct "Ha" as %Ha; simpl in Ha; subst; wp_rec.
     - wp_match. iApply ("HΦ" $! 0%nat); done.
     - destruct Ha as [lv' [Hlv Hlcoh]]; subst.
-      wp_match. wp_proj. wp_bind (length _).
+      wp_match. wp_proj. wp_bind (list_length _).
       iApply ("IH" $! _ _ Hlcoh). iNext. iIntros; simpl.
       wp_op. iSpecialize ("HΦ" $! (1 + v)%nat).
       rewrite Nat2Z.inj_add. iApply "HΦ"; by auto.
   Qed.
 
-  Lemma list_iter_spec {A} ip (l : list A) lv handler P Φ Ψ
+  Lemma wp_list_iter {A} ip (l : list A) lv handler P Φ Ψ
         (toval : A -> base_lang.val) :
     (∀ (a : A),
         {{{ ⌜a ∈ l⌝ ∗ P ∗ Φ a }}}
           (Val handler) (toval a) @[ip]
         {{{v, RET v; P ∗ Ψ a }}}) -∗
-    {{{ ⌜is_List (map (λ a, toval a) l) lv⌝ ∗ P ∗ [∗ list] a∈l, Φ a }}}
-      iter (Val handler) lv @[ip]
+    {{{ ⌜is_list (map (λ a, toval a) l) lv⌝ ∗ P ∗ [∗ list] a∈l, Φ a }}}
+      list_iter (Val handler) lv @[ip]
     {{{ RET #(); P ∗ [∗ list] a ∈ l, Ψ a }}}.
   Proof.
-    rewrite /iter.
+    rewrite /list_iter.
     iInduction l as [|a l'] "IH" forall (lv);
     iIntros "#Helem"; iIntros (Φ') "!# (Ha & HP & Hl) HΦ";
     iDestruct "Ha" as %Ha; simpl in Ha; subst; wp_pures.
@@ -215,19 +209,19 @@ Section List_specs.
     iNext. iIntros "(HP & Hl)". iApply "HΦ". iFrame.
   Qed.
 
-  Lemma list_fold_spec {A} ip handler (l : list A)  acc lv P Φ Ψ
+  Lemma wp_list_fold {A} ip handler (l : list A)  acc lv P Φ Ψ
         (toval : A -> base_lang.val) :
     (∀ (a : A) acc lacc lrem,
         {{{ ⌜l = lacc ++ a :: lrem⌝ ∗ P lacc acc ∗ Φ a }}}
           (Val handler) (Val acc) (toval a) @[ip]
         {{{v, RET v; P (lacc ++ [a]) v ∗ Ψ a }}}) -∗
-    {{{ ⌜is_List (map (λ a, toval a) l) lv⌝ ∗ P [] acc ∗ [∗ list] a∈l, Φ a }}}
-      fold handler acc lv @[ip]
+    {{{ ⌜is_list (map (λ a, toval a) l) lv⌝ ∗ P [] acc ∗ [∗ list] a∈l, Φ a }}}
+      list_fold handler acc lv @[ip]
     {{{v, RET v; P l v ∗ [∗ list] a∈l, Ψ a }}}.
   Proof.
     iIntros "#Hcl". iIntros (Ξ) "!# (Hl & Hacc & HΦ) HΞ".
     change l with ([] ++ l) at 1 4.
-    generalize (@Datatypes.nil A) at 1 3 4 as lproc => lproc.
+    generalize (@nil A) at 1 3 4 as lproc => lproc.
     iInduction l as [|x l] "IHl" forall (Ξ lproc acc lv) "Hacc Hl HΞ".
     - iDestruct "Hl" as %?; simpl in *; simplify_eq.
       wp_rec. wp_pures. iApply "HΞ".
@@ -244,15 +238,15 @@ Section List_specs.
       iApply "HΞ"; iFrame.
   Qed.
 
-  Lemma list_fold_spec'_generalized {A} ip handler (l lp : list A) acc lv P Φ Ψ
+  Lemma wp_list_fold_generalized' {A} ip handler (l lp : list A) acc lv P Φ Ψ
         (toval : A -> base_lang.val) :
     □ (∀ (a : A) acc lacc lrem, (P lacc acc None (a::lrem) -∗ P lacc acc (Some a) lrem))%I -∗
       (∀ (a : A) acc lacc lrem,
           {{{ ⌜lp ++ l = lacc ++ a :: lrem⌝ ∗ P lacc acc (Some a) lrem ∗ Φ a }}}
             (Val handler) (Val acc) (toval a) @[ip]
           {{{v, RET v; P (lacc ++ [a]) v None lrem ∗ Ψ a }}}) -∗
-    {{{ ⌜is_List (map (λ a, toval a) l) lv⌝ ∗ P lp acc None l ∗ [∗ list] a∈l, Φ a }}}
-      fold (Val handler) (Val acc) (Val lv) @[ip]
+    {{{ ⌜is_list (map (λ a, toval a) l) lv⌝ ∗ P lp acc None l ∗ [∗ list] a∈l, Φ a }}}
+      list_fold (Val handler) (Val acc) (Val lv) @[ip]
     {{{v, RET v; P (lp ++ l) v None [] ∗ [∗ list] a∈l, Ψ a }}}.
   Proof.
     iIntros "#Hvs #Hcl". iIntros (Ξ) "!# (Hl & Hacc & HΦ) HΞ".
@@ -273,25 +267,25 @@ Section List_specs.
       iApply "HΞ"; iFrame.
   Qed.
 
-  Lemma list_fold_spec' {A} ip handler (l : list A) acc lv P Φ Ψ
+  Lemma wo_list_fold' {A} ip handler (l : list A) acc lv P Φ Ψ
         (toval : A -> base_lang.val) :
     □ (∀ (a : A) acc lacc lrem, (P lacc acc None (a::lrem) -∗ P lacc acc (Some a) lrem))%I -∗
       (∀ (a : A) acc lacc lrem,
           {{{ ⌜l = lacc ++ a :: lrem⌝ ∗ P lacc acc (Some a) lrem ∗ Φ a }}}
             (Val handler) (Val acc) (toval a) @[ip]
           {{{v, RET v; P (lacc ++ [a]) v None lrem ∗ Ψ a }}}) -∗
-    {{{ ⌜is_List (map (λ a, toval a) l) lv⌝ ∗ P [] acc None l ∗ [∗ list] a∈l, Φ a }}}
-      fold (Val handler) (Val acc) lv @[ip]
+    {{{ ⌜is_list (map (λ a, toval a) l) lv⌝ ∗ P [] acc None l ∗ [∗ list] a∈l, Φ a }}}
+      list_fold (Val handler) (Val acc) lv @[ip]
     {{{v, RET v; P l v None [] ∗ [∗ list] a∈l, Ψ a }}}.
   Proof.
     iIntros "#Hvs #Hcl".
-    iApply (list_fold_spec'_generalized _ handler l [] with "[-]"); eauto.
+    iApply (wp_list_fold_generalized' _ handler l [] with "[-]"); eauto.
   Qed.
 
-  Lemma list_sub_spec ip k l lv  :
-    {{{ ⌜is_List l lv⌝ }}}
-      sub #k lv @[ip]
-    {{{ v, RET v; ⌜is_List (take k l) v ⌝}}}.
+  Lemma wp_list_sub ip k l lv  :
+    {{{ ⌜is_list l lv⌝ }}}
+      list_sub #k lv @[ip]
+    {{{ v, RET v; ⌜is_list (take k l) v ⌝}}}.
   Proof.
    iIntros (Φ) "Hcoh HΦ".
    iInduction l as [|a l'] "IH" forall (k lv Φ);
@@ -301,17 +295,17 @@ Section List_specs.
    - iApply "HΦ"; by rewrite take_nil.
    - iApply "HΦ". assert (k = O) as H1 by lia. by rewrite H1 firstn_O.
    - destruct Hcoh as [lv' [Hlv Hlcoh]]; subst.
-     wp_match. wp_proj. wp_bind (sub _ _). wp_op.
+     wp_match. wp_proj. wp_bind (list_sub _ _). wp_op.
      destruct k as [|k]; first done.
      assert (((Z.of_nat (S k)) - 1)%Z = Z.of_nat k) as -> by lia.
      iApply ("IH" $! k _ _ Hlcoh). iIntros (tl Hcoh_tl).
-     iNext. wp_pures. rewrite firstn_cons. by wp_apply (list_cons_spec).
+     iNext. wp_pures. rewrite firstn_cons. by wp_apply (wp_list_cons).
   Qed.
 
-  Lemma list_nth_spec ip (i: nat) l lv  :
-   {{{ ⌜is_List l lv⌝ }}}
-      nth (Val lv) #i @[ip]
-    {{{ v, RET v; (⌜v = NONEV⌝ ∧ ⌜Datatypes.length l <= i⌝) ∨
+  Lemma wp_list_nth ip (i: nat) l lv  :
+   {{{ ⌜is_list l lv⌝ }}}
+      list_nth (Val lv) #i @[ip]
+    {{{ v, RET v; (⌜v = NONEV⌝ ∧ ⌜length l <= i⌝) ∨
               ⌜∃ r, v = SOMEV r ∧ nth_error l i = Some r⌝ }}}.
   Proof.
     iIntros (Φ) "Ha HΦ".
@@ -330,30 +324,30 @@ Section List_specs.
         * iApply "HΦ"; try eauto with lia.
   Qed.
 
-  Lemma list_nth_spec_some ip (i: nat) l lv  :
-    {{{  ⌜is_List l lv ∧ i < Datatypes.length l⌝  }}}
-      nth (Val lv) #i @[ip]
+  Lemma wp_list_nth_some ip (i: nat) l lv  :
+    {{{  ⌜is_list l lv ∧ i < length l⌝  }}}
+      list_nth (Val lv) #i @[ip]
     {{{ v, RET v; ⌜∃ r, v = SOMEV r ∧ nth_error l i = Some r⌝ }}}.
   Proof.
     iIntros (Φ (Hcoh & Hi)) "HΦ".
-    iApply (list_nth_spec $! Hcoh).
+    iApply (wp_list_nth $! Hcoh).
     iIntros (v [H | H]); first eauto with lia.
     by iApply "HΦ".
   Qed.
 
-  Lemma find_remove_spec {A} ip (l : list A) lv (Ψ : A → iProp Σ)
+  Lemma wp_find_remove {A} ip (l : list A) lv (Ψ : A → iProp Σ)
         (fv : base_lang.val) (toval : A → base_lang.val) :
     (∀ (a : A) av,
         {{{ ⌜av = toval a⌝ }}}
           fv av @[ip]
         {{{ (b : bool), RET #b; if b then Ψ a else True }}}) -∗
-    {{{ ⌜is_List (map (λ a, toval a) l) lv⌝ }}}
-      find_remove fv lv @[ip]
+    {{{ ⌜is_list (map (λ a, toval a) l) lv⌝ }}}
+      list_find_remove fv lv @[ip]
     {{{ v, RET v; ⌜v = NONEV⌝ ∨
                        ∃ e lv' l1 l2,
                          ⌜l = l1 ++ e :: l2 ∧
                          v = SOMEV (toval e, lv') ∧
-                         is_List (map (λ a, toval a) (l1 ++ l2)) lv'⌝
+                         is_list (map (λ a, toval a) (l1 ++ l2)) lv'⌝
                          ∗ Ψ e}}}.
   Proof.
     iIntros "#Hf" (Φ).
@@ -369,7 +363,7 @@ Section List_specs.
       iApply "HΦ".
       iRight; iExists _, _, [], _; eauto. }
     wp_pures.
-    wp_bind (find_remove _ _).
+    wp_bind (list_find_remove _ _).
     iApply ("IH" with "[//]").
     iIntros "!>" (w) "[->| He] /="; wp_pures.
     { iApply "HΦ".
@@ -377,39 +371,39 @@ Section List_specs.
     iDestruct "He" as (e lv'' l1 l2) "[He HHΨ]".
     iDestruct "He" as %(-> & -> & Hlv'').
     wp_pures.
-    wp_bind (cons _ _). iApply list_cons_spec; first done.
+    wp_bind (list_cons _ _). iApply wp_list_cons; first done.
     iIntros "!>" (v Hcoh) "/=". wp_pures.
     iApply "HΦ". iRight.
     iExists _, _, (_ :: _), _; eauto.
   Qed.
 
-  Lemma list_rev_aux_spec ip l lM r rM:
-   {{{ ⌜is_List lM l ∧ is_List rM r⌝ }}}
-     rev_aux (Val l) (Val r) @[ip]
-   {{{ v, RET v; ⌜is_List (rev_append lM rM) v⌝ }}}.
+  Local Lemma wp_list_rev_aux ip l lM r rM:
+   {{{ ⌜is_list lM l ∧ is_list rM r⌝ }}}
+     list_rev_aux (Val l) (Val r) @[ip]
+   {{{ v, RET v; ⌜is_list (rev_append lM rM) v⌝ }}}.
   Proof.
     iIntros (? [Hl Hr]) "H".
     iInduction lM as [|a lM] "IH" forall (l r rM Hl Hr).
-    - simpl in *; subst. rewrite /rev_aux. wp_pures. by iApply "H".
+    - simpl in *; subst. rewrite /list_rev_aux. wp_pures. by iApply "H".
     - destruct Hl as [l' [Hl'eq Hl']]; subst.
       wp_rec; wp_pures.
-      wp_apply list_cons_spec; first done.
+      wp_apply wp_list_cons; first done.
       iIntros (w Hw).
       wp_pures. by iApply "IH".
  Qed.
 
-  Lemma list_rev_spec ip l lM :
-    {{{ ⌜is_List lM l⌝ }}}
-      rev (Val l) @[ip]
-    {{{ v, RET v; ⌜is_List (reverse lM) v⌝ }}}.
+  Lemma wp_list_rev ip l lM :
+    {{{ ⌜is_list lM l⌝ }}}
+      list_rev (Val l) @[ip]
+    {{{ v, RET v; ⌜is_list (reverse lM) v⌝ }}}.
   Proof.
-    iIntros (??) "H". rewrite /rev. wp_pures.
-    by iApply (list_rev_aux_spec _ _ _ NONEV []).
+    iIntros (??) "H". rewrite /list_rev. wp_pures.
+    by iApply (wp_list_rev_aux _ _ _ NONEV []).
   Qed.
 
-  Lemma list_is_empty_spec ip l v :
-    {{{ ⌜is_List l v⌝ }}}
-      is_empty v @[ip]
+  Lemma wp_list_is_empty l v ip :
+    {{{ ⌜is_list l v⌝ }}}
+      list_is_empty v @[ip]
     {{{ v, RET #v;
         ⌜v = match l with [] => true | _ => false end⌝ }}}.
   Proof.
@@ -418,20 +412,23 @@ Section List_specs.
     - destruct Hl as [? [-> _]]. wp_pures. by iApply "HΦ".
   Qed.
 
-  Lemma is_List_eq lM :
-    ∀ l1 l2, is_List lM l1 → is_List lM l2 → l1 = l2.
+  Lemma is_list_eq lM :
+    ∀ l1 l2, is_list lM l1 → is_list lM l2 → l1 = l2.
   Proof. induction lM; intros []; naive_solver eauto with f_equal. Qed.
 
-  Lemma is_List_inv_l l:
-    ∀ lM1 lM2, is_List lM1 l → lM1 = lM2 → is_List lM2 l.
+  Lemma is_list_inv_l l:
+    ∀ lM1 lM2, is_list lM1 l → lM1 = lM2 → is_list lM2 l.
   Proof. by intros ? ? ? <-. Qed.
 
-  Lemma is_List_snoc lM x : ∃ lv, is_List (lM ++ [x]) lv.
+  Lemma is_list_snoc lM x : ∃ lv, is_list (lM ++ [x]) lv.
   Proof. induction lM; naive_solver eauto. Qed.
 
   Definition str_val (l : list string) : list base_lang.val :=
     map (λ (str : string), #str) l.
 
-End List_specs.
+End list_specs.
 
-Infix "::" := List.cons (at level 60, right associativity) : expr_scope.
+Notation "[ ]" := list_nil (format "[ ]") : expr_scope.
+Infix "::" := list_cons (at level 60, right associativity) : expr_scope.
+Notation "[ x ; y ; .. ; z ]" := (list_cons x (list_cons y .. (list_cons z nil) ..)) : expr_scope.
+
