theories/aneris_lang/lib/vector_clock/vector_clock.v
@@ -8,18 +8,18 @@ Section vect_code.
 
   Definition vect_make : base_lang.val :=
     rec: "vect_make" "len" "init" :=
-      if: "len" = #0 then List.nil
-      else List.cons "init" ("vect_make" ("len" - #1) "init").
+      if: "len" = #0 then list_nil
+      else list_cons "init" ("vect_make" ("len" - #1) "init").
 
   Definition vect_nth : base_lang.val :=
-    λ: "vec" "i", unSOME (List.nth "vec" "i").
+    λ: "vec" "i", unSOME (list_nth "vec" "i").
 
   Definition vect_update : base_lang.val :=
     rec: "vect_update" "vec" "i" "v" :=
       match: "vec" with
         SOME "a" =>
-           if: "i" = #0 then List.cons "v" (List.tail "vec")
-           else List.cons (Fst "a") ("vect_update" (Snd "a") ("i" - #1) "v")
+           if: "i" = #0 then list_cons "v" (list_tail "vec")
+           else list_cons (Fst "a") ("vect_update" (Snd "a") ("i" - #1) "v")
         | NONE => NONE
       end.
 
@@ -36,7 +36,7 @@ Section vect_code.
                        (Fst "a1" ≤ Fst "a2") && "vect_leq" (Snd "a1") (Snd "a2")
                      | NONE => #false
                      end
-      | NONE => List.is_empty "v2"
+      | NONE => list_is_empty "v2"
       end.
 
   Definition vect_applicable : base_lang.val :=
@@ -52,7 +52,7 @@ Section vect_code.
                        && "vect_applicable" ("j" + #1) (Snd "a1") (Snd "a2")
                      | NONE => #false
                      end
-       | NONE => List.is_empty "v2"
+       | NONE => list_is_empty "v2"
        end) #0 "v1" "v2".
 
   Definition vect_serialize : base_lang.val :=
@@ -71,8 +71,8 @@ Section vect_code.
             let: "length" := UnOp StringLength "s" in
             let: "start" := "i" + #1 in
             "vect_deserialize" (Substring "s" "start" ("length" - "start")) in
-          List.cons "x" "tail"
-      | NONE => List.nil
+          list_cons "x" "tail"
+      | NONE => list_nil
       end.
 
 End vect_code.
@@ -81,7 +81,7 @@ Section vect_specs.
   Context `{!anerisG Mdl Σ}.
 
   Definition is_vc (v : base_lang.val) (t : vector_clock) :=
-    is_List (map (λ (n : nat), #n) t) v.
+    is_list (map (λ (n : nat), #n) t) v.
 
   Lemma vector_clock_to_val_is_vc t : is_vc (vector_clock_to_val t) t.
   Proof.
@@ -95,14 +95,14 @@ Section vect_specs.
     intros [? [-> ?]]; erewrite IHt; done.
   Qed.
 
-  Lemma vect_make_spec ip len (init : nat):
+  Lemma wp_vect_make ip len (init : nat):
     {{{ True }}}
       vect_make #len #init @[ip]
     {{{ v, RET v; ⌜is_vc v (replicate len init)⌝ }}}.
   Proof.
     revert len. iLöb as "IH". iIntros (len Φ) "_ HΦ".
     wp_rec. wp_pures. case_bool_decide; wp_if.
-    - iApply list_nil_spec; [done|].
+    - iApply wp_list_nil; [done|].
       iNext; iIntros (v) "%".
       iApply "HΦ".
       assert (len = 0%nat) by lia; simplify_eq. done.
@@ -110,7 +110,7 @@ Section vect_specs.
       assert (((Z.of_nat len) - 1)%Z = Z.of_nat (len - 1)) as -> by lia.
       iApply "IH"; first done.
       iNext. iIntros (? Hcoh) "/=".
-      iApply list_cons_spec; [done|].
+      iApply wp_list_cons; [done|].
       iNext; iIntros (w) "%".
       iApply "HΦ". iPureIntro.
       assert (∃ n, len = S n) as [m Hlen'].
@@ -119,26 +119,26 @@ Section vect_specs.
       by assert (m = (len - 1)%nat) as -> by lia.
   Qed.
 
-  Lemma vect_nth_spec ip v (i : nat) t :
+  Lemma wp_vect_nth ip v (i : nat) t :
     i < length t →
     {{{ ⌜is_vc v t⌝ }}}
       vect_nth v #i @[ip]
     {{{ v, RET v; ⌜∃ (j : nat), v = #j ∧ t !! i = Some j⌝ }}}.
   Proof.
     iIntros (Hlen Φ Hcoh) "HΦ".
-    wp_rec. wp_pures. wp_bind (List.nth _ _).
-    iApply (list_nth_spec_some).
+    wp_rec. wp_pures. wp_bind (list_nth _ _).
+    iApply (wp_list_nth_some).
     { iPureIntro. split; eauto.
       rewrite map_length. lia. }
     iNext; iIntros (w [k [-> H]]) "/=".
-    iApply unSOME_spec; first done.
+    iApply wp_unSOME; first done.
     iNext; iIntros "_".
     iApply "HΦ". iPureIntro.
     apply nth_error_lookup in H.
     by apply map_lookup_Some in H.
   Qed.
 
-  Lemma vect_update_spec ip v t (i j : nat) :
+  Lemma wp_vect_update ip v t (i j : nat) :
     i < length t →
     {{{ ⌜is_vc v t⌝ }}}
       vect_update v #i #j @[ip]
@@ -150,11 +150,11 @@ Section vect_specs.
     - rewrite Hcoh. wp_pures. by iApply "HΦ".
     - destruct Hcoh as [k [H' Hl']].
       rewrite H'. wp_pures. case_bool_decide; wp_pures.
-      + wp_bind (List.tail _).
-        iApply (list_tail_spec _ _ (#x :: (map (λ n : nat, #n) t))).
+      + wp_bind (list_tail _).
+        iApply (wp_list_tail _ _ (#x :: (map (λ n : nat, #n) t))).
         { iPureIntro. eexists; eauto. }
         iNext. iIntros (tm Htm) "/=".
-        iApply (list_cons_spec $! Htm).
+        iApply (wp_list_cons $! Htm).
         iNext. iIntros (u Hu) "/=".
         iApply "HΦ"; iPureIntro.
         assert (i = 0)%nat as -> by lia.
@@ -167,12 +167,12 @@ Section vect_specs.
         destruct i; first done; simpl.
         rewrite !Nat.sub_0_r.
         iNext; iIntros (tm Htm) "/=". wp_pures.
-        iApply (list_cons_spec $! Htm).
+        iApply (wp_list_cons $! Htm).
         iNext; iIntros (? ?).
         by iApply "HΦ".
   Qed.
 
-  Lemma vect_inc_spec ip v t (i j : nat) :
+  Lemma wp_vect_inc ip v t (i j : nat) :
     i < length t →
     t !! i = Some j →
     {{{ ⌜is_vc v t⌝ }}}
@@ -181,14 +181,14 @@ Section vect_specs.
   Proof.
     iIntros (Hi Hj Φ Hcoh) "HΦ".
     wp_rec. wp_pures. wp_bind (vect_nth _ _).
-    iApply vect_nth_spec; eauto.
+    iApply wp_vect_nth; eauto.
     iNext; iIntros (w [j' [-> Hj']]) "/=". simplify_eq. wp_pures.
     assert (((Z.of_nat j) + 1)%Z = Z.of_nat (S j)) as -> by lia.
     rewrite /incr_time Hj /=.
-    iApply vect_update_spec; eauto.
+    iApply wp_vect_update; eauto.
   Qed.
 
-  Lemma vect_leq_spec ip v1 v2 (l1 l2 : list nat) :
+  Lemma wp_vect_leq ip v1 v2 (l1 l2 : list nat) :
     {{{ ⌜is_vc v1 l1⌝ ∗ ⌜is_vc v2 l2⌝ }}}
       vect_leq v1 v2 @[ip]
     {{{ v, RET #v; ⌜v = bool_decide (vector_clock_le l1 l2)⌝ }}}.
@@ -200,13 +200,13 @@ Section vect_specs.
       destruct l2.
       + rewrite Hl2.
         wp_pures.
-        iApply (list_is_empty_spec _ []); first done.
+        iApply (wp_list_is_empty []); first done.
         iNext; iIntros (v ->).
         iApply "HΦ".
         rewrite bool_decide_eq_true_2; last constructor; done.
       + destruct Hl2 as (? & -> & Hl2).
         wp_pures.
-        iApply (list_is_empty_spec _ (_ :: _));
+        iApply (wp_list_is_empty (_ :: _));
           first by iPureIntro; eexists; eauto.
         iNext; iIntros (v ->).
         iApply "HΦ".
@@ -235,7 +235,7 @@ Section vect_specs.
           inversion 1; simplify_eq. lia.
   Qed.
 
-  Lemma vect_applicable_spec ip v1 v2 (l1 l2 : list nat) (i : nat) :
+  Lemma wp_vect_applicable ip v1 v2 (l1 l2 : list nat) (i : nat) :
     {{{ ⌜is_vc v1 l1⌝ ∗ ⌜is_vc v2 l2⌝ }}}
       vect_applicable v1 v2 #i @[ip]
     {{{ (b : bool), RET #b;
@@ -290,7 +290,7 @@ Section vect_specs.
     iInduction l1 as [|x1 l1] "IHl1" forall (j v1 v2 Hl1 l2 Hl2).
     { rewrite Hl1.
       wp_pures.
-      iApply list_is_empty_spec; first done.
+      iApply wp_list_is_empty; first done.
       iNext. iIntros (? ->).
       destruct l2; simpl; last by iExists false.
       iExists true.
@@ -371,7 +371,6 @@ End vect_specs.
 
 Arguments is_vc : simpl never.
 
-
 Fixpoint vc_to_string (l : vector_clock) : string :=
   match l with
   | [] => ""
@@ -384,7 +383,7 @@ Definition vc_valid_val (v : base_lang.val) :=
 Definition vc_is_ser (v : base_lang.val) (s : string) :=
   ∃ l, is_vc v l ∧ s = vc_to_string l.
 
-Definition vect_serialize_spec `{!anerisG Mdl Σ} ip v:
+Definition wp_vect_serialize `{!anerisG Mdl Σ} ip v:
   {{{ ⌜vc_valid_val v⌝ }}}
     vect_serialize v @[ip]
   {{{ s, RET #s; ⌜vc_is_ser v s⌝ }}}.
@@ -407,7 +406,7 @@ Proof.
     iPureIntro; eexists (_ :: _); simpl; split; first eexists _; eauto.
 Qed.
 
-Definition vect_deserialize_spec `{!anerisG Mdl Σ} ip v s:
+Definition wp_vect_deserialize `{!anerisG Mdl Σ} ip v s:
   {{{ ⌜vc_is_ser v s⌝ }}}
     vect_deserialize #s @[ip]
   {{{ RET v; True }}}.
@@ -428,7 +427,7 @@ Proof.
     rewrite substring_0_length_append.
     wp_pure _.
     { simpl. rewrite ZOfString_inv //. }
-    wp_apply unSOME_spec; [done|].
+    wp_apply wp_unSOME; [done|].
     iIntros "_ /=". wp_pures.
     rewrite !length_app.
     wp_substring;
@@ -443,9 +442,9 @@ Proof.
     rewrite substring_0_length.
     wp_apply "IH"; [iPureIntro; exists l; done|].
     iIntros "_ /=". wp_pures.
-    wp_apply list_cons_spec; first done.
+    wp_apply wp_list_cons; first done.
     iIntros (? [u [-> Hu]]).
-    rewrite (is_List_eq _ _ _ Hl Hu).
+    rewrite (is_list_eq _ _ _ Hl Hu).
     iApply "HΦ"; done.
 Qed.
 
@@ -454,5 +453,5 @@ Definition vc_serialization : serialization :=
      DBS_ser := vect_serialize;
      DBS_deser := vect_deserialize;
      DBS_is_ser := vc_is_ser;
-     DBS_ser_spec := @vect_serialize_spec;
-     DBS_deser_spec := @vect_deserialize_spec; |}.
+     DBS_ser_spec := @wp_vect_serialize;
+     DBS_deser_spec := @wp_vect_deserialize; |}.
